Impl/CommitterCommitModel.i.dfy
@@ -1,4 +1,4 @@
-include "CommitterModel.i.dfy"
+// include "CommitterModel.i.dfy"
 // include "StateModel.i.dfy"
 include "IOModel.i.dfy"
 include "../lib/DataStructures/LinearMutableMap.i.dfy"
@@ -16,7 +16,8 @@ module CommitterCommitModel {
   import opened DiskOpModel
   import SectorType
 
-  import opened CommitterModel
+  import LinearMutableMap
+  // import opened CommitterModel
   // import opened StateModel
   import opened IOModel
 
@@ -151,687 +152,687 @@ module CommitterCommitModel {
       else a + b
   }
 
-  function {:opaque} WriteOutJournal(cm: CM, io: IO)
-      : (res : (CM, IO))
-  requires io.IOInit?
-  requires CommitterModel.WF(cm)
-  requires JournalistModel.I(cm.journalist).inMemoryJournalFrozen != []
-        || JournalistModel.I(cm.journalist).inMemoryJournal != []
-  {
-    var writtenJournalLen :=
-        JournalistModel.getWrittenJournalLen(cm.journalist);
-
-    var doingFrozen :=
-      JournalistModel.hasFrozenJournal(cm.journalist);
-
-    var (journalist', j) :=
-      if doingFrozen then
-        JournalistModel.packageFrozenJournal(cm.journalist)
-      else
-        JournalistModel.packageInMemoryJournal(cm.journalist);
-
-    var start := start_pos_add(
-        cm.superblock.journalStart,
-        writtenJournalLen);
-
-    var len := |j| as uint64 / 4096;
-
-    var contiguous := start + len <= NumJournalBlocks();
-
-    var io' := if contiguous then
-      IOReqWrite(io.id, D.ReqWrite(JournalPoint(start), j))
-    else (
-      var cut := (NumJournalBlocks() - start) * 4096;
-      IOReqWrite2(io.id, io.id2,
-          D.ReqWrite(JournalPoint(start), j[..cut]),
-          D.ReqWrite(JournalPoint(0), j[cut..]))
-    );
-
-    var outstandingJournalWrites' := if contiguous
-        then cm.outstandingJournalWrites + {io.id}
-        else cm.outstandingJournalWrites + {io.id, io.id2};
-
-    var frozenJournalPosition' := if doingFrozen
-      then JournalistModel.getWrittenJournalLen(journalist')
-      else cm.frozenJournalPosition;
-
-    var syncReqs' := if doingFrozen
-      then cm.syncReqs
-      else SyncReqs3to2(cm.syncReqs);
-
-    var cm' := cm
-      .(outstandingJournalWrites := outstandingJournalWrites')
-      .(journalist := journalist')
-      .(frozenJournalPosition := frozenJournalPosition')
-      .(syncReqs := syncReqs');
-
-    (cm', io')
-  }
-
-  lemma WriteOutJournalCorrect(cm: CM, io: IO)
-  requires WriteOutJournal.requires(cm, io)
-  requires cm.superblockWrite.None?
-  ensures var (cm', io') := WriteOutJournal(cm, io);
-    && CommitterModel.WF(cm')
-    && ValidDiskOp(diskOp(io'))
-    && IDiskOp(diskOp(io')).bdop.NoDiskOp?
-    && JC.Next(
-        CommitterModel.I(cm),
-        CommitterModel.I(cm'),
-        IDiskOp(diskOp(io')).jdop,
-        JournalInternalOp)
-  {
-    var (cm', io') := WriteOutJournal(cm, io);
-    reveal_WriteOutJournal();
-
-    var writtenJournalLen :=
-        JournalistModel.getWrittenJournalLen(cm.journalist);
-
-    var doingFrozen :=
-      JournalistModel.hasFrozenJournal(cm.journalist);
-
-    var (journalist', j) :=
-      if doingFrozen then
-        JournalistModel.packageFrozenJournal(cm.journalist)
-      else
-        JournalistModel.packageInMemoryJournal(cm.journalist);
-
-    var start := start_pos_add(
-        cm.superblock.journalStart,
-        writtenJournalLen);
-
-    var jr := JournalRangeOfByteSeq(j).value;
-    var len := |j| as uint64 / 4096;
-    var contiguous := start + len <= NumJournalBlocks();
-
-    assert |jr| == len as int;
-
-    if contiguous {
-      assert LocOfReqWrite(diskOp(io').reqWrite)
-          == JournalRangeLocation(start, len);
-      assert ValidDiskOp(diskOp(io'));
-    } else {
-      assert LocOfReqWrite(diskOp(io').reqWrite1)
-          == JournalRangeLocation(start, NumJournalBlocks() - start);
-      assert LocOfReqWrite(diskOp(io').reqWrite2)
-          == JournalRangeLocation(0, len - (NumJournalBlocks() - start));
-      JournalBytesSplit(j, len as int,
-          NumJournalBlocks() as int - start as int);
-      assert ValidDiskOp(diskOp(io'));
-    }
-
-    SyncReqs3to2Correct(cm.syncReqs);
-
-    assert JC.WriteBackJournalReq(
-        CommitterModel.I(cm),
-        CommitterModel.I(cm'),
-        IDiskOp(diskOp(io')).jdop,
-        JournalInternalOp,
-        jr);
-    assert JC.NextStep(
-        CommitterModel.I(cm),
-        CommitterModel.I(cm'),
-        IDiskOp(diskOp(io')).jdop,
-        JournalInternalOp,
-        JC.WriteBackJournalReqStep(jr));
-  }
-
-  predicate writeOutSuperblockAdvanceLog(cm: CM, io: IO,
-      cm': CM, io': IO)
-  requires io.IOInit?
-  requires CommitterModel.WF(cm)
-  {
-    var writtenJournalLen :=
-        JournalistModel.getWrittenJournalLen(cm.journalist);
-    var newSuperblock := SectorType.Superblock(
-      JC.IncrementSuperblockCounter(cm.superblock.counter),
-      cm.superblock.journalStart,
-      writtenJournalLen,
-      cm.superblock.indirectionTableLoc
-    );
-
-    var loc := if cm.whichSuperblock == 0 then Superblock2Location() else Superblock1Location();
-
-    && cm'.superblockWrite.Some?
-    && var id := cm'.superblockWrite.value;
-
-    && RequestWrite(io, loc, SSM.SectorSuperblock(newSuperblock),
-        id, io')
-    && cm' == cm
-      .(newSuperblock := Some(newSuperblock))
-      .(superblockWrite := Some(id))
-      .(commitStatus := JC.CommitAdvanceLog)
-  }
-
-  lemma writeOutSuperblockAdvanceLogCorrect(cm: CM, io: IO,
-      cm': CM, io': IO)
-  requires io.IOInit?
-  requires CommitterModel.WF(cm)
-  requires writeOutSuperblockAdvanceLog(cm, io, cm', io')
-  requires cm.status == StatusReady
-  requires cm.commitStatus.CommitNone?
-  requires cm.outstandingJournalWrites == {}
-  requires JournalistModel.I(cm.journalist).inMemoryJournalFrozen == []
-  ensures CommitterModel.WF(cm')
-  ensures ValidDiskOp(diskOp(io'))
-  ensures IDiskOp(diskOp(io')).bdop.NoDiskOp?
-  ensures JC.Next(
-        CommitterModel.I(cm),
-        CommitterModel.I(cm'),
-        IDiskOp(diskOp(io')).jdop,
-        JournalInternalOp)
-  {
-    var writtenJournalLen :=
-        JournalistModel.getWrittenJournalLen(cm.journalist);
-    var newSuperblock := SectorType.Superblock(
-      JC.IncrementSuperblockCounter(cm.superblock.counter),
-      cm.superblock.journalStart,
-      writtenJournalLen,
-      cm.superblock.indirectionTableLoc
-    );
-    assert JC.WFSuperblock(newSuperblock);
-
-    var loc := if cm.whichSuperblock == 0 then Superblock2Location() else Superblock1Location();
-
-    var id := cm'.superblockWrite.value;
-
-    RequestWriteCorrect(io, loc, SSM.SectorSuperblock(newSuperblock),
-        id, io');
-
-    assert ValidDiskOp(diskOp(io'));
-
-    assert JC.WriteBackSuperblockReq_AdvanceLog(
-        CommitterModel.I(cm),
-        CommitterModel.I(cm'),
-        IDiskOp(diskOp(io')).jdop,
-        JournalInternalOp);
-    assert JC.NextStep(
-        CommitterModel.I(cm),
-        CommitterModel.I(cm'),
-        IDiskOp(diskOp(io')).jdop,
-        JournalInternalOp,
-        JC.WriteBackSuperblockReq_AdvanceLog_Step);
-  }
-
-  predicate {:opaque} writeOutSuperblockAdvanceLocation(cm: CM, io: IO,
-      cm': CM, io': IO)
-  requires io.IOInit?
-  requires CommitterModel.Inv(cm)
-  requires cm.status == StatusReady
-  requires cm.frozenLoc.Some?
-  {
-    var writtenJournalLen :=
-        JournalistModel.getWrittenJournalLen(cm.journalist);
-    var newSuperblock := SectorType.Superblock(
-      JC.IncrementSuperblockCounter(cm.superblock.counter),
-      start_pos_add(
-          cm.superblock.journalStart,
-          cm.frozenJournalPosition),
-      writtenJournalLen - cm.frozenJournalPosition,
-      cm.frozenLoc.value
-    );
-
-    var loc := if cm.whichSuperblock == 0 then Superblock2Location() else Superblock1Location();
-
-    && cm'.superblockWrite.Some?
-    && var id := cm'.superblockWrite.value;
-
-    && RequestWrite(io, loc, SSM.SectorSuperblock(newSuperblock),
-        id, io')
-    && cm' == cm
-      .(newSuperblock := Some(newSuperblock))
-      .(superblockWrite := Some(id))
-      .(commitStatus := JC.CommitAdvanceLocation)
-  }
-
-  lemma writeOutSuperblockAdvanceLocationCorrect(cm: CM, io: IO,
-      cm': CM, io': IO)
-  requires io.IOInit?
-  requires CommitterModel.Inv(cm)
-  requires cm.status == StatusReady
-  requires cm.frozenLoc.Some?
-  requires cm.commitStatus.CommitNone?
-  requires cm.outstandingJournalWrites == {}
-  requires writeOutSuperblockAdvanceLocation(cm, io, cm', io')
-  requires JournalistModel.I(cm.journalist).inMemoryJournalFrozen == []
-  ensures CommitterModel.WF(cm')
-  ensures ValidDiskOp(diskOp(io'))
-  ensures IDiskOp(diskOp(io')).bdop.NoDiskOp?
-  ensures JC.Next(
-        CommitterModel.I(cm),
-        CommitterModel.I(cm'),
-        IDiskOp(diskOp(io')).jdop,
-        JournalInternalOp)
-  {
-    reveal_writeOutSuperblockAdvanceLocation();
-
-    var writtenJournalLen :=
-        JournalistModel.getWrittenJournalLen(cm.journalist);
-    var newSuperblock := SectorType.Superblock(
-      JC.IncrementSuperblockCounter(cm.superblock.counter),
-      start_pos_add(
-          cm.superblock.journalStart,
-          cm.frozenJournalPosition) as uint64,
-      (writtenJournalLen - cm.frozenJournalPosition) as uint64,
-      cm.frozenLoc.value
-    );
-    assert JC.WFSuperblock(newSuperblock);
-
-    var loc := if cm.whichSuperblock == 0 then Superblock2Location() else Superblock1Location();
-
-    var id := cm'.superblockWrite.value;
-
-    RequestWriteCorrect(io, loc, SSM.SectorSuperblock(newSuperblock),
-        id, io');
-
-    assert ValidDiskOp(diskOp(io'));
-
-    assert JC.WriteBackSuperblockReq_AdvanceLocation(
-        CommitterModel.I(cm),
-        CommitterModel.I(cm'),
-        IDiskOp(diskOp(io')).jdop,
-        JournalInternalOp);
-    assert JC.NextStep(
-        CommitterModel.I(cm),
-        CommitterModel.I(cm'),
-        IDiskOp(diskOp(io')).jdop,
-        JournalInternalOp,
-        JC.WriteBackSuperblockReq_AdvanceLocation_Step);
-  }
-
-  function {:opaque} freeze(cm: CM) : (cm': CM)
-  requires CommitterModel.WF(cm)
-  {
-    var writtenJournalLen :=
-        JournalistModel.getWrittenJournalLen(cm.journalist);
-    cm.(frozenLoc := None)
-      .(journalist := JournalistModel.freeze(cm.journalist))
-      .(frozenJournalPosition := writtenJournalLen)
-      .(isFrozen := true)
-      .(syncReqs := SyncReqs3to2(cm.syncReqs))
-  }
-
-  lemma freezeCorrect(cm: CM)
-  requires CommitterModel.WF(cm)
-  requires cm.superblockWrite.None?
-
-  // Mostly we'll probably just do this with cm.frozenLoc == None
-  // but more generally we can do it whenever we have:
-  requires cm.status == StatusReady
-  requires cm.frozenLoc != Some(cm.superblock.indirectionTableLoc)
-  requires JournalistModel.I(cm.journalist).replayJournal == []
-
-  ensures var cm' := freeze(cm);
-    && CommitterModel.WF(cm')
-    && JC.Next(
-        CommitterModel.I(cm),
-        CommitterModel.I(cm'),
-        JournalDisk.NoDiskOp,
-        FreezeOp)
-  {
-    reveal_freeze();
-    var cm' := freeze(cm);
-    SyncReqs3to2Correct(cm.syncReqs);
-
-    assert JC.Freeze(
-        CommitterModel.I(cm),
-        CommitterModel.I(cm'),
-        JournalDisk.NoDiskOp,
-        FreezeOp);
-    assert JC.NextStep(
-        CommitterModel.I(cm),
-        CommitterModel.I(cm'),
-        JournalDisk.NoDiskOp,
-        FreezeOp,
-        JC.FreezeStep);
-  }
-
-  function {:opaque} receiveFrozenLoc(
-      cm: CM, loc: Location) : (cm': CM)
-  {
-    cm.(frozenLoc := Some(loc))
-  }
-
-  lemma receiveFrozenLocCorrect(cm: CM, loc: Location)
-  requires CommitterModel.WF(cm)
-  requires cm.status == StatusReady
-  requires cm.isFrozen
-  requires !cm.frozenLoc.Some?
-  requires ValidIndirectionTableLocation(loc)
-
-  ensures var cm' := receiveFrozenLoc(cm, loc);
-    && CommitterModel.WF(cm')
-    && JC.Next(
-        CommitterModel.I(cm),
-        CommitterModel.I(cm'),
-        JournalDisk.NoDiskOp,
-        SendFrozenLocOp(loc))
-  {
-    reveal_receiveFrozenLoc();
-    var cm' := receiveFrozenLoc(cm, loc);
-    assert JC.ReceiveFrozenLoc(
-        CommitterModel.I(cm),
-        CommitterModel.I(cm'),
-        JournalDisk.NoDiskOp,
-        SendFrozenLocOp(loc));
-    assert JC.NextStep(
-        CommitterModel.I(cm),
-        CommitterModel.I(cm'),
-        JournalDisk.NoDiskOp,
-        SendFrozenLocOp(loc),
-        JC.ReceiveFrozenLocStep);
-  }
-
-  // == pushSync ==
-
-  function {:opaque} freeId<A>(syncReqs: LinearMutableMap.LinearHashMap<A>) : (id: uint64)
-  requires LinearMutableMap.Inv(syncReqs)
-  ensures id != 0 ==> id !in syncReqs.contents
-  {
-    var maxId := LinearMutableMap.MaxKey(syncReqs);
-    if maxId == 0xffff_ffff_ffff_ffff then (
-      0
-    ) else (
-      maxId + 1
-    )
-  }
-
-  function pushSync(cm: CM) : (CM, uint64)
-  requires CommitterModel.WF(cm)
-  {
-    var id := freeId(cm.syncReqs);
-    if id == 0 || cm.syncReqs.count as int >= 0x1_0000_0000_0000_0000 / 8 then (
-      (cm, 0)
-    ) else (
-      var cm' := cm.(syncReqs := LinearMutableMap.Insert(cm.syncReqs, id, JC.State3));
-      (cm', id)
-    )
-  }
-
-  lemma pushSyncCorrect(cm: CM)
-  requires CommitterModel.WF(cm)
-
-  ensures var (cm', id) := pushSync(cm);
-    && CommitterModel.WF(cm')
-    && JC.Next(
-        CommitterModel.I(cm),
-        CommitterModel.I(cm'),
-        JournalDisk.NoDiskOp,
-        if id == 0 then JournalInternalOp else PushSyncOp(id as int))
-  {
-    var (cm', id) := pushSync(cm);
-    if id == 0 || cm.syncReqs.count as int >= 0x1_0000_0000_0000_0000 / 8 {
-      assert JC.NoOp(
-          CommitterModel.I(cm),
-          CommitterModel.I(cm'),
-          JournalDisk.NoDiskOp,
-          JournalInternalOp);
-      assert JC.NextStep(
-          CommitterModel.I(cm),
-          CommitterModel.I(cm'),
-          JournalDisk.NoDiskOp,
-          JournalInternalOp,
-          JC.NoOpStep);
-    } else {
-      assert JC.PushSyncReq(
-          CommitterModel.I(cm),
-          CommitterModel.I(cm'),
-          JournalDisk.NoDiskOp,
-          PushSyncOp(id as int), id);
-      assert JC.NextStep(
-          CommitterModel.I(cm),
-          CommitterModel.I(cm'),
-          JournalDisk.NoDiskOp,
-          PushSyncOp(id as int),
-          JC.PushSyncReqStep(id));
-    }
-  }
-
-  // == popSync ==
-
-  function {:opaque} popSync(cm: CM, id: uint64) : (cm' : CM)
-  requires CommitterModel.WF(cm)
-  {
-    cm.(syncReqs := LinearMutableMap.Remove(cm.syncReqs, id))
-  }
-
-  lemma popSyncCorrect(cm: CM, id: uint64)
-  requires CommitterModel.WF(cm)
-  requires id in cm.syncReqs.contents
-  requires cm.syncReqs.contents[id] == JC.State1
-  ensures var cm' := popSync(cm, id);
-    && CommitterModel.WF(cm')
-    && JC.Next(
-        CommitterModel.I(cm),
-        CommitterModel.I(cm'),
-        JournalDisk.NoDiskOp,
-        PopSyncOp(id as int))
-  {
-    var cm' := popSync(cm, id);
-    reveal_popSync();
-    assert JC.PopSyncReq(
-        CommitterModel.I(cm),
-        CommitterModel.I(cm'),
-        JournalDisk.NoDiskOp,
-        PopSyncOp(id as int), id);
-    assert JC.NextStep(
-        CommitterModel.I(cm),
-        CommitterModel.I(cm'),
-        JournalDisk.NoDiskOp,
-        PopSyncOp(id as int),
-        JC.PopSyncReqStep(id));
-  }
-
-  // == AdvanceLog ==
-
-  predicate {:opaque} tryAdvanceLog(cm: CM, io: IO,
-      cm': CM, io': IO)
-  requires CommitterModel.WF(cm)
-  requires io.IOInit?
-  {
-    var hasFrozen := JournalistModel.hasFrozenJournal(cm.journalist);
-    var hasInMem := JournalistModel.hasInMemoryJournal(cm.journalist);
-    if cm.superblockWrite.None? then (
-      if hasFrozen || hasInMem then (
-        (cm', io') == WriteOutJournal(cm, io)
-      ) else if cm.outstandingJournalWrites == {} then (
-        writeOutSuperblockAdvanceLog(cm, io, cm', io')
-      ) else (
-        && cm' == cm
-        && io' == io
-      )
-    ) else (
-      && cm' == cm
-      && io' == io
-    )
-  }
-
-  lemma tryAdvanceLogCorrect(cm: CM, io: IO,
-      cm': CM, io': IO)
-  requires CommitterModel.Inv(cm)
-  requires io.IOInit?
-  requires cm.status.StatusReady?
-  requires tryAdvanceLog(cm, io, cm', io')
-  ensures CommitterModel.WF(cm')
-  ensures ValidDiskOp(diskOp(io'))
-  ensures IDiskOp(diskOp(io')).bdop.NoDiskOp?
-  ensures JC.Next(
-        CommitterModel.I(cm),
-        CommitterModel.I(cm'),
-        IDiskOp(diskOp(io')).jdop,
-        JournalInternalOp)
-  {
-    reveal_tryAdvanceLog();
-    var hasFrozen := JournalistModel.hasFrozenJournal(cm.journalist);
-    var hasInMem := JournalistModel.hasInMemoryJournal(cm.journalist);
-    if cm.superblockWrite.None? {
-      if hasFrozen || hasInMem {
-        WriteOutJournalCorrect(cm, io);
-      } else if (cm.outstandingJournalWrites == {}) {
-        writeOutSuperblockAdvanceLogCorrect(cm, io, cm', io');
-      } else {
-        assert JC.NoOp( CommitterModel.I(cm), CommitterModel.I(cm'), JournalDisk.NoDiskOp, JournalInternalOp);
-        assert JC.NextStep( CommitterModel.I(cm), CommitterModel.I(cm'), JournalDisk.NoDiskOp, JournalInternalOp, JC.NoOpStep);
-      }
-    } else {
-      assert JC.NoOp( CommitterModel.I(cm), CommitterModel.I(cm'), JournalDisk.NoDiskOp, JournalInternalOp);
-      assert JC.NextStep( CommitterModel.I(cm), CommitterModel.I(cm'), JournalDisk.NoDiskOp, JournalInternalOp, JC.NoOpStep);
-    }
-  }
-
-  predicate {:opaque} tryAdvanceLocation(cm: CM, io: IO,
-      cm': CM, io': IO)
-  requires CommitterModel.Inv(cm)
-  requires io.IOInit?
-  requires cm.status == StatusReady
-  requires cm.frozenLoc.Some?
-  {
-    var hasFrozen := JournalistModel.hasFrozenJournal(cm.journalist);
-    var hasInMem := JournalistModel.hasInMemoryJournal(cm.journalist);
-    if cm.superblockWrite.None? then (
-      if hasFrozen || hasInMem then (
-        (cm', io') == WriteOutJournal(cm, io)
-      ) else if cm.outstandingJournalWrites == {} then (
-        writeOutSuperblockAdvanceLocation(cm, io, cm', io')
-      ) else (
-        && cm' == cm
-        && io' == io
-      )
-    ) else (
-      && cm' == cm
-      && io' == io
-    )
-  }
-
-  lemma tryAdvanceLocationCorrect(cm: CM, io: IO,
-      cm': CM, io': IO)
-  requires CommitterModel.Inv(cm)
-  requires io.IOInit?
-  requires cm.status.StatusReady?
-  requires cm.frozenLoc.Some?
-  requires tryAdvanceLocation(cm, io, cm', io')
-  ensures CommitterModel.WF(cm')
-  ensures ValidDiskOp(diskOp(io'))
-  ensures IDiskOp(diskOp(io')).bdop.NoDiskOp?
-  ensures JC.Next(
-        CommitterModel.I(cm),
-        CommitterModel.I(cm'),
-        IDiskOp(diskOp(io')).jdop,
-        JournalInternalOp)
-  {
-    reveal_tryAdvanceLocation();
-    var hasFrozen := JournalistModel.hasFrozenJournal(cm.journalist);
-    var hasInMem := JournalistModel.hasInMemoryJournal(cm.journalist);
-    if cm.superblockWrite.None? {
-      if hasFrozen || hasInMem {
-        WriteOutJournalCorrect(cm, io);
-      } else if (cm.outstandingJournalWrites == {}) {
-        writeOutSuperblockAdvanceLocationCorrect(cm, io, cm', io');
-      } else {
-        assert JC.NoOp( CommitterModel.I(cm), CommitterModel.I(cm'), JournalDisk.NoDiskOp, JournalInternalOp);
-        assert JC.NextStep( CommitterModel.I(cm), CommitterModel.I(cm'), JournalDisk.NoDiskOp, JournalInternalOp, JC.NoOpStep);
-      }
-    } else {
-      assert JC.NoOp( CommitterModel.I(cm), CommitterModel.I(cm'), JournalDisk.NoDiskOp, JournalInternalOp);
-      assert JC.NextStep( CommitterModel.I(cm), CommitterModel.I(cm'), JournalDisk.NoDiskOp, JournalInternalOp, JC.NoOpStep);
-    }
-  }
-
-  function {:opaque} writeBackSuperblockResp(
-      cm: CommitterModel.CM) : CommitterModel.CM
-  requires CommitterModel.Inv(cm)
-  {
-    if cm.status.StatusReady? &&
-        cm.commitStatus.CommitAdvanceLocation? then (
-      cm.(superblockWrite := None)
-        .(superblock := cm.newSuperblock.value)
-        .(newSuperblock := None)
-        .(whichSuperblock := if cm.whichSuperblock == 0 then 1 else 0)
-        .(syncReqs := SyncReqs2to1(cm.syncReqs))
-        .(journalist :=
-            JournalistModel.updateWrittenJournalLen(
-              cm.journalist,
-              JournalistModel.getWrittenJournalLen(cm.journalist)
-                - cm.frozenJournalPosition
-            )
-         )
-        .(frozenJournalPosition := 0)
-        .(frozenLoc := None)
-        .(isFrozen := false)
-        .(commitStatus := JC.CommitNone)
-    )
-    else if cm.status.StatusReady? &&
-        cm.commitStatus.CommitAdvanceLog? then (
-      cm.(superblockWrite := None)
-        .(superblock := cm.newSuperblock.value)
-        .(newSuperblock := None)
-        .(whichSuperblock := if cm.whichSuperblock == 0 then 1 else 0)
-        .(syncReqs := SyncReqs2to1(cm.syncReqs))
-        .(commitStatus := JC.CommitNone)
-    )
-    else (
-      cm
-    )
-  }
-
-  lemma writeBackSuperblockRespCorrect(
-      cm: CommitterModel.CM, io: IO)
-  requires CommitterModel.Inv(cm)
-  requires ValidDiskOp(diskOp(io))
-  requires IDiskOp(diskOp(io)).jdop.RespWriteSuperblockOp?
-  requires Some(io.id) == cm.superblockWrite
-  ensures var cm' := writeBackSuperblockResp(cm);
-    && CommitterModel.WF(cm')
-    && JC.Next(
-        CommitterModel.I(cm),
-        CommitterModel.I(cm'),
-        IDiskOp(diskOp(io)).jdop,
-        if cm.status.StatusReady? && cm.commitStatus.CommitAdvanceLocation? then CleanUpOp else JournalInternalOp
-    )
-  {
-    reveal_writeBackSuperblockResp();
-    var cm' := writeBackSuperblockResp(cm);
-    SyncReqs2to1Correct(cm.syncReqs);
-    if cm.status.StatusReady? &&
-        cm.commitStatus.CommitAdvanceLocation? {
-      assert JC.WriteBackSuperblockResp(
-          CommitterModel.I(cm),
-          CommitterModel.I(cm'),
-          IDiskOp(diskOp(io)).jdop,
-          CleanUpOp);
-      assert JC.NextStep(
-          CommitterModel.I(cm),
-          CommitterModel.I(cm'),
-          IDiskOp(diskOp(io)).jdop,
-          CleanUpOp,
-          JC.WriteBackSuperblockRespStep);
-    }
-    else if cm.status.StatusReady? &&
-        cm.commitStatus.CommitAdvanceLog? {
-      assert JC.WriteBackSuperblockResp(
-          CommitterModel.I(cm),
-          CommitterModel.I(cm'),
-          IDiskOp(diskOp(io)).jdop,
-          JournalInternalOp);
-      assert JC.NextStep(
-          CommitterModel.I(cm),
-          CommitterModel.I(cm'),
-          IDiskOp(diskOp(io)).jdop,
-          JournalInternalOp,
-          JC.WriteBackSuperblockRespStep);
-    }
-    else {
-      assert JC.NoOp(
-          CommitterModel.I(cm),
-          CommitterModel.I(cm'),
-          IDiskOp(diskOp(io)).jdop,
-          JournalInternalOp);
-      assert JC.NextStep(
-          CommitterModel.I(cm),
-          CommitterModel.I(cm'),
-          IDiskOp(diskOp(io)).jdop,
-          JournalInternalOp,
-          JC.NoOpStep);
-    }
-  }
+  // function {:opaque} WriteOutJournal(cm: CM, io: IO)
+  //     : (res : (CM, IO))
+  // requires io.IOInit?
+  // requires CommitterModel.WF(cm)
+  // requires JournalistModel.I(cm.journalist).inMemoryJournalFrozen != []
+  //       || JournalistModel.I(cm.journalist).inMemoryJournal != []
+  // {
+  //   var writtenJournalLen :=
+  //       JournalistModel.getWrittenJournalLen(cm.journalist);
+
+  //   var doingFrozen :=
+  //     JournalistModel.hasFrozenJournal(cm.journalist);
+
+  //   var (journalist', j) :=
+  //     if doingFrozen then
+  //       JournalistModel.packageFrozenJournal(cm.journalist)
+  //     else
+  //       JournalistModel.packageInMemoryJournal(cm.journalist);
+
+  //   var start := start_pos_add(
+  //       cm.superblock.journalStart,
+  //       writtenJournalLen);
+
+  //   var len := |j| as uint64 / 4096;
+
+  //   var contiguous := start + len <= NumJournalBlocks();
+
+  //   var io' := if contiguous then
+  //     IOReqWrite(io.id, D.ReqWrite(JournalPoint(start), j))
+  //   else (
+  //     var cut := (NumJournalBlocks() - start) * 4096;
+  //     IOReqWrite2(io.id, io.id2,
+  //         D.ReqWrite(JournalPoint(start), j[..cut]),
+  //         D.ReqWrite(JournalPoint(0), j[cut..]))
+  //   );
+
+  //   var outstandingJournalWrites' := if contiguous
+  //       then cm.outstandingJournalWrites + {io.id}
+  //       else cm.outstandingJournalWrites + {io.id, io.id2};
+
+  //   var frozenJournalPosition' := if doingFrozen
+  //     then JournalistModel.getWrittenJournalLen(journalist')
+  //     else cm.frozenJournalPosition;
+
+  //   var syncReqs' := if doingFrozen
+  //     then cm.syncReqs
+  //     else SyncReqs3to2(cm.syncReqs);
+
+  //   var cm' := cm
+  //     .(outstandingJournalWrites := outstandingJournalWrites')
+  //     .(journalist := journalist')
+  //     .(frozenJournalPosition := frozenJournalPosition')
+  //     .(syncReqs := syncReqs');
+
+  //   (cm', io')
+  // }
+
+  // lemma WriteOutJournalCorrect(cm: CM, io: IO)
+  // requires WriteOutJournal.requires(cm, io)
+  // requires cm.superblockWrite.None?
+  // ensures var (cm', io') := WriteOutJournal(cm, io);
+  //   && CommitterModel.WF(cm')
+  //   && ValidDiskOp(diskOp(io'))
+  //   && IDiskOp(diskOp(io')).bdop.NoDiskOp?
+  //   && JC.Next(
+  //       CommitterModel.I(cm),
+  //       CommitterModel.I(cm'),
+  //       IDiskOp(diskOp(io')).jdop,
+  //       JournalInternalOp)
+  // {
+  //   var (cm', io') := WriteOutJournal(cm, io);
+  //   reveal_WriteOutJournal();
+
+  //   var writtenJournalLen :=
+  //       JournalistModel.getWrittenJournalLen(cm.journalist);
+
+  //   var doingFrozen :=
+  //     JournalistModel.hasFrozenJournal(cm.journalist);
+
+  //   var (journalist', j) :=
+  //     if doingFrozen then
+  //       JournalistModel.packageFrozenJournal(cm.journalist)
+  //     else
+  //       JournalistModel.packageInMemoryJournal(cm.journalist);
+
+  //   var start := start_pos_add(
+  //       cm.superblock.journalStart,
+  //       writtenJournalLen);
+
+  //   var jr := JournalRangeOfByteSeq(j).value;
+  //   var len := |j| as uint64 / 4096;
+  //   var contiguous := start + len <= NumJournalBlocks();
+
+  //   assert |jr| == len as int;
+
+  //   if contiguous {
+  //     assert LocOfReqWrite(diskOp(io').reqWrite)
+  //         == JournalRangeLocation(start, len);
+  //     assert ValidDiskOp(diskOp(io'));
+  //   } else {
+  //     assert LocOfReqWrite(diskOp(io').reqWrite1)
+  //         == JournalRangeLocation(start, NumJournalBlocks() - start);
+  //     assert LocOfReqWrite(diskOp(io').reqWrite2)
+  //         == JournalRangeLocation(0, len - (NumJournalBlocks() - start));
+  //     JournalBytesSplit(j, len as int,
+  //         NumJournalBlocks() as int - start as int);
+  //     assert ValidDiskOp(diskOp(io'));
+  //   }
+
+  //   SyncReqs3to2Correct(cm.syncReqs);
+
+  //   assert JC.WriteBackJournalReq(
+  //       CommitterModel.I(cm),
+  //       CommitterModel.I(cm'),
+  //       IDiskOp(diskOp(io')).jdop,
+  //       JournalInternalOp,
+  //       jr);
+  //   assert JC.NextStep(
+  //       CommitterModel.I(cm),
+  //       CommitterModel.I(cm'),
+  //       IDiskOp(diskOp(io')).jdop,
+  //       JournalInternalOp,
+  //       JC.WriteBackJournalReqStep(jr));
+  // }
+
+  // predicate writeOutSuperblockAdvanceLog(cm: CM, io: IO,
+  //     cm': CM, io': IO)
+  // requires io.IOInit?
+  // requires CommitterModel.WF(cm)
+  // {
+  //   var writtenJournalLen :=
+  //       JournalistModel.getWrittenJournalLen(cm.journalist);
+  //   var newSuperblock := SectorType.Superblock(
+  //     JC.IncrementSuperblockCounter(cm.superblock.counter),
+  //     cm.superblock.journalStart,
+  //     writtenJournalLen,
+  //     cm.superblock.indirectionTableLoc
+  //   );
+
+  //   var loc := if cm.whichSuperblock == 0 then Superblock2Location() else Superblock1Location();
+
+  //   && cm'.superblockWrite.Some?
+  //   && var id := cm'.superblockWrite.value;
+
+  //   && RequestWrite(io, loc, SSM.SectorSuperblock(newSuperblock),
+  //       id, io')
+  //   && cm' == cm
+  //     .(newSuperblock := Some(newSuperblock))
+  //     .(superblockWrite := Some(id))
+  //     .(commitStatus := JC.CommitAdvanceLog)
+  // }
+
+  // lemma writeOutSuperblockAdvanceLogCorrect(cm: CM, io: IO,
+  //     cm': CM, io': IO)
+  // requires io.IOInit?
+  // requires CommitterModel.WF(cm)
+  // requires writeOutSuperblockAdvanceLog(cm, io, cm', io')
+  // requires cm.status == StatusReady
+  // requires cm.commitStatus.CommitNone?
+  // requires cm.outstandingJournalWrites == {}
+  // requires JournalistModel.I(cm.journalist).inMemoryJournalFrozen == []
+  // ensures CommitterModel.WF(cm')
+  // ensures ValidDiskOp(diskOp(io'))
+  // ensures IDiskOp(diskOp(io')).bdop.NoDiskOp?
+  // ensures JC.Next(
+  //       CommitterModel.I(cm),
+  //       CommitterModel.I(cm'),
+  //       IDiskOp(diskOp(io')).jdop,
+  //       JournalInternalOp)
+  // {
+  //   var writtenJournalLen :=
+  //       JournalistModel.getWrittenJournalLen(cm.journalist);
+  //   var newSuperblock := SectorType.Superblock(
+  //     JC.IncrementSuperblockCounter(cm.superblock.counter),
+  //     cm.superblock.journalStart,
+  //     writtenJournalLen,
+  //     cm.superblock.indirectionTableLoc
+  //   );
+  //   assert JC.WFSuperblock(newSuperblock);
+
+  //   var loc := if cm.whichSuperblock == 0 then Superblock2Location() else Superblock1Location();
+
+  //   var id := cm'.superblockWrite.value;
+
+  //   RequestWriteCorrect(io, loc, SSM.SectorSuperblock(newSuperblock),
+  //       id, io');
+
+  //   assert ValidDiskOp(diskOp(io'));
+
+  //   assert JC.WriteBackSuperblockReq_AdvanceLog(
+  //       CommitterModel.I(cm),
+  //       CommitterModel.I(cm'),
+  //       IDiskOp(diskOp(io')).jdop,
+  //       JournalInternalOp);
+  //   assert JC.NextStep(
+  //       CommitterModel.I(cm),
+  //       CommitterModel.I(cm'),
+  //       IDiskOp(diskOp(io')).jdop,
+  //       JournalInternalOp,
+  //       JC.WriteBackSuperblockReq_AdvanceLog_Step);
+  // }
+
+  // predicate {:opaque} writeOutSuperblockAdvanceLocation(cm: CM, io: IO,
+  //     cm': CM, io': IO)
+  // requires io.IOInit?
+  // requires CommitterModel.Inv(cm)
+  // requires cm.status == StatusReady
+  // requires cm.frozenLoc.Some?
+  // {
+  //   var writtenJournalLen :=
+  //       JournalistModel.getWrittenJournalLen(cm.journalist);
+  //   var newSuperblock := SectorType.Superblock(
+  //     JC.IncrementSuperblockCounter(cm.superblock.counter),
+  //     start_pos_add(
+  //         cm.superblock.journalStart,
+  //         cm.frozenJournalPosition),
+  //     writtenJournalLen - cm.frozenJournalPosition,
+  //     cm.frozenLoc.value
+  //   );
+
+  //   var loc := if cm.whichSuperblock == 0 then Superblock2Location() else Superblock1Location();
+
+  //   && cm'.superblockWrite.Some?
+  //   && var id := cm'.superblockWrite.value;
+
+  //   && RequestWrite(io, loc, SSM.SectorSuperblock(newSuperblock),
+  //       id, io')
+  //   && cm' == cm
+  //     .(newSuperblock := Some(newSuperblock))
+  //     .(superblockWrite := Some(id))
+  //     .(commitStatus := JC.CommitAdvanceLocation)
+  // }
+
+  // lemma writeOutSuperblockAdvanceLocationCorrect(cm: CM, io: IO,
+  //     cm': CM, io': IO)
+  // requires io.IOInit?
+  // requires CommitterModel.Inv(cm)
+  // requires cm.status == StatusReady
+  // requires cm.frozenLoc.Some?
+  // requires cm.commitStatus.CommitNone?
+  // requires cm.outstandingJournalWrites == {}
+  // requires writeOutSuperblockAdvanceLocation(cm, io, cm', io')
+  // requires JournalistModel.I(cm.journalist).inMemoryJournalFrozen == []
+  // ensures CommitterModel.WF(cm')
+  // ensures ValidDiskOp(diskOp(io'))
+  // ensures IDiskOp(diskOp(io')).bdop.NoDiskOp?
+  // ensures JC.Next(
+  //       CommitterModel.I(cm),
+  //       CommitterModel.I(cm'),
+  //       IDiskOp(diskOp(io')).jdop,
+  //       JournalInternalOp)
+  // {
+  //   reveal_writeOutSuperblockAdvanceLocation();
+
+  //   var writtenJournalLen :=
+  //       JournalistModel.getWrittenJournalLen(cm.journalist);
+  //   var newSuperblock := SectorType.Superblock(
+  //     JC.IncrementSuperblockCounter(cm.superblock.counter),
+  //     start_pos_add(
+  //         cm.superblock.journalStart,
+  //         cm.frozenJournalPosition) as uint64,
+  //     (writtenJournalLen - cm.frozenJournalPosition) as uint64,
+  //     cm.frozenLoc.value
+  //   );
+  //   assert JC.WFSuperblock(newSuperblock);
+
+  //   var loc := if cm.whichSuperblock == 0 then Superblock2Location() else Superblock1Location();
+
+  //   var id := cm'.superblockWrite.value;
+
+  //   RequestWriteCorrect(io, loc, SSM.SectorSuperblock(newSuperblock),
+  //       id, io');
+
+  //   assert ValidDiskOp(diskOp(io'));
+
+  //   assert JC.WriteBackSuperblockReq_AdvanceLocation(
+  //       CommitterModel.I(cm),
+  //       CommitterModel.I(cm'),
+  //       IDiskOp(diskOp(io')).jdop,
+  //       JournalInternalOp);
+  //   assert JC.NextStep(
+  //       CommitterModel.I(cm),
+  //       CommitterModel.I(cm'),
+  //       IDiskOp(diskOp(io')).jdop,
+  //       JournalInternalOp,
+  //       JC.WriteBackSuperblockReq_AdvanceLocation_Step);
+  // }
+
+  // function {:opaque} freeze(cm: CM) : (cm': CM)
+  // requires CommitterModel.WF(cm)
+  // {
+  //   var writtenJournalLen :=
+  //       JournalistModel.getWrittenJournalLen(cm.journalist);
+  //   cm.(frozenLoc := None)
+  //     .(journalist := JournalistModel.freeze(cm.journalist))
+  //     .(frozenJournalPosition := writtenJournalLen)
+  //     .(isFrozen := true)
+  //     .(syncReqs := SyncReqs3to2(cm.syncReqs))
+  // }
+
+  // lemma freezeCorrect(cm: CM)
+  // requires CommitterModel.WF(cm)
+  // requires cm.superblockWrite.None?
+
+  // // Mostly we'll probably just do this with cm.frozenLoc == None
+  // // but more generally we can do it whenever we have:
+  // requires cm.status == StatusReady
+  // requires cm.frozenLoc != Some(cm.superblock.indirectionTableLoc)
+  // requires JournalistModel.I(cm.journalist).replayJournal == []
+
+  // ensures var cm' := freeze(cm);
+  //   && CommitterModel.WF(cm')
+  //   && JC.Next(
+  //       CommitterModel.I(cm),
+  //       CommitterModel.I(cm'),
+  //       JournalDisk.NoDiskOp,
+  //       FreezeOp)
+  // {
+  //   reveal_freeze();
+  //   var cm' := freeze(cm);
+  //   SyncReqs3to2Correct(cm.syncReqs);
+
+  //   assert JC.Freeze(
+  //       CommitterModel.I(cm),
+  //       CommitterModel.I(cm'),
+  //       JournalDisk.NoDiskOp,
+  //       FreezeOp);
+  //   assert JC.NextStep(
+  //       CommitterModel.I(cm),
+  //       CommitterModel.I(cm'),
+  //       JournalDisk.NoDiskOp,
+  //       FreezeOp,
+  //       JC.FreezeStep);
+  // }
+
+  // function {:opaque} receiveFrozenLoc(
+  //     cm: CM, loc: Location) : (cm': CM)
+  // {
+  //   cm.(frozenLoc := Some(loc))
+  // }
+
+  // lemma receiveFrozenLocCorrect(cm: CM, loc: Location)
+  // requires CommitterModel.WF(cm)
+  // requires cm.status == StatusReady
+  // requires cm.isFrozen
+  // requires !cm.frozenLoc.Some?
+  // requires ValidIndirectionTableLocation(loc)
+
+  // ensures var cm' := receiveFrozenLoc(cm, loc);
+  //   && CommitterModel.WF(cm')
+  //   && JC.Next(
+  //       CommitterModel.I(cm),
+  //       CommitterModel.I(cm'),
+  //       JournalDisk.NoDiskOp,
+  //       SendFrozenLocOp(loc))
+  // {
+  //   reveal_receiveFrozenLoc();
+  //   var cm' := receiveFrozenLoc(cm, loc);
+  //   assert JC.ReceiveFrozenLoc(
+  //       CommitterModel.I(cm),
+  //       CommitterModel.I(cm'),
+  //       JournalDisk.NoDiskOp,
+  //       SendFrozenLocOp(loc));
+  //   assert JC.NextStep(
+  //       CommitterModel.I(cm),
+  //       CommitterModel.I(cm'),
+  //       JournalDisk.NoDiskOp,
+  //       SendFrozenLocOp(loc),
+  //       JC.ReceiveFrozenLocStep);
+  // }
+
+  // // == pushSync ==
+
+  // function {:opaque} freeId<A>(syncReqs: LinearMutableMap.LinearHashMap<A>) : (id: uint64)
+  // requires LinearMutableMap.Inv(syncReqs)
+  // ensures id != 0 ==> id !in syncReqs.contents
+  // {
+  //   var maxId := LinearMutableMap.MaxKey(syncReqs);
+  //   if maxId == 0xffff_ffff_ffff_ffff then (
+  //     0
+  //   ) else (
+  //     maxId + 1
+  //   )
+  // }
+
+  // function pushSync(cm: CM) : (CM, uint64)
+  // requires CommitterModel.WF(cm)
+  // {
+  //   var id := freeId(cm.syncReqs);
+  //   if id == 0 || cm.syncReqs.count as int >= 0x1_0000_0000_0000_0000 / 8 then (
+  //     (cm, 0)
+  //   ) else (
+  //     var cm' := cm.(syncReqs := LinearMutableMap.Insert(cm.syncReqs, id, JC.State3));
+  //     (cm', id)
+  //   )
+  // }
+
+  // lemma pushSyncCorrect(cm: CM)
+  // requires CommitterModel.WF(cm)
+
+  // ensures var (cm', id) := pushSync(cm);
+  //   && CommitterModel.WF(cm')
+  //   && JC.Next(
+  //       CommitterModel.I(cm),
+  //       CommitterModel.I(cm'),
+  //       JournalDisk.NoDiskOp,
+  //       if id == 0 then JournalInternalOp else PushSyncOp(id as int))
+  // {
+  //   var (cm', id) := pushSync(cm);
+  //   if id == 0 || cm.syncReqs.count as int >= 0x1_0000_0000_0000_0000 / 8 {
+  //     assert JC.NoOp(
+  //         CommitterModel.I(cm),
+  //         CommitterModel.I(cm'),
+  //         JournalDisk.NoDiskOp,
+  //         JournalInternalOp);
+  //     assert JC.NextStep(
+  //         CommitterModel.I(cm),
+  //         CommitterModel.I(cm'),
+  //         JournalDisk.NoDiskOp,
+  //         JournalInternalOp,
+  //         JC.NoOpStep);
+  //   } else {
+  //     assert JC.PushSyncReq(
+  //         CommitterModel.I(cm),
+  //         CommitterModel.I(cm'),
+  //         JournalDisk.NoDiskOp,
+  //         PushSyncOp(id as int), id);
+  //     assert JC.NextStep(
+  //         CommitterModel.I(cm),
+  //         CommitterModel.I(cm'),
+  //         JournalDisk.NoDiskOp,
+  //         PushSyncOp(id as int),
+  //         JC.PushSyncReqStep(id));
+  //   }
+  // }
+
+  // // == popSync ==
+
+  // function {:opaque} popSync(cm: CM, id: uint64) : (cm' : CM)
+  // requires CommitterModel.WF(cm)
+  // {
+  //   cm.(syncReqs := LinearMutableMap.Remove(cm.syncReqs, id))
+  // }
+
+  // lemma popSyncCorrect(cm: CM, id: uint64)
+  // requires CommitterModel.WF(cm)
+  // requires id in cm.syncReqs.contents
+  // requires cm.syncReqs.contents[id] == JC.State1
+  // ensures var cm' := popSync(cm, id);
+  //   && CommitterModel.WF(cm')
+  //   && JC.Next(
+  //       CommitterModel.I(cm),
+  //       CommitterModel.I(cm'),
+  //       JournalDisk.NoDiskOp,
+  //       PopSyncOp(id as int))
+  // {
+  //   var cm' := popSync(cm, id);
+  //   reveal_popSync();
+  //   assert JC.PopSyncReq(
+  //       CommitterModel.I(cm),
+  //       CommitterModel.I(cm'),
+  //       JournalDisk.NoDiskOp,
+  //       PopSyncOp(id as int), id);
+  //   assert JC.NextStep(
+  //       CommitterModel.I(cm),
+  //       CommitterModel.I(cm'),
+  //       JournalDisk.NoDiskOp,
+  //       PopSyncOp(id as int),
+  //       JC.PopSyncReqStep(id));
+  // }
+
+  // // == AdvanceLog ==
+
+  // predicate {:opaque} tryAdvanceLog(cm: CM, io: IO,
+  //     cm': CM, io': IO)
+  // requires CommitterModel.WF(cm)
+  // requires io.IOInit?
+  // {
+  //   var hasFrozen := JournalistModel.hasFrozenJournal(cm.journalist);
+  //   var hasInMem := JournalistModel.hasInMemoryJournal(cm.journalist);
+  //   if cm.superblockWrite.None? then (
+  //     if hasFrozen || hasInMem then (
+  //       (cm', io') == WriteOutJournal(cm, io)
+  //     ) else if cm.outstandingJournalWrites == {} then (
+  //       writeOutSuperblockAdvanceLog(cm, io, cm', io')
+  //     ) else (
+  //       && cm' == cm
+  //       && io' == io
+  //     )
+  //   ) else (
+  //     && cm' == cm
+  //     && io' == io
+  //   )
+  // }
+
+  // lemma tryAdvanceLogCorrect(cm: CM, io: IO,
+  //     cm': CM, io': IO)
+  // requires CommitterModel.Inv(cm)
+  // requires io.IOInit?
+  // requires cm.status.StatusReady?
+  // requires tryAdvanceLog(cm, io, cm', io')
+  // ensures CommitterModel.WF(cm')
+  // ensures ValidDiskOp(diskOp(io'))
+  // ensures IDiskOp(diskOp(io')).bdop.NoDiskOp?
+  // ensures JC.Next(
+  //       CommitterModel.I(cm),
+  //       CommitterModel.I(cm'),
+  //       IDiskOp(diskOp(io')).jdop,
+  //       JournalInternalOp)
+  // {
+  //   reveal_tryAdvanceLog();
+  //   var hasFrozen := JournalistModel.hasFrozenJournal(cm.journalist);
+  //   var hasInMem := JournalistModel.hasInMemoryJournal(cm.journalist);
+  //   if cm.superblockWrite.None? {
+  //     if hasFrozen || hasInMem {
+  //       WriteOutJournalCorrect(cm, io);
+  //     } else if (cm.outstandingJournalWrites == {}) {
+  //       writeOutSuperblockAdvanceLogCorrect(cm, io, cm', io');
+  //     } else {
+  //       assert JC.NoOp( CommitterModel.I(cm), CommitterModel.I(cm'), JournalDisk.NoDiskOp, JournalInternalOp);
+  //       assert JC.NextStep( CommitterModel.I(cm), CommitterModel.I(cm'), JournalDisk.NoDiskOp, JournalInternalOp, JC.NoOpStep);
+  //     }
+  //   } else {
+  //     assert JC.NoOp( CommitterModel.I(cm), CommitterModel.I(cm'), JournalDisk.NoDiskOp, JournalInternalOp);
+  //     assert JC.NextStep( CommitterModel.I(cm), CommitterModel.I(cm'), JournalDisk.NoDiskOp, JournalInternalOp, JC.NoOpStep);
+  //   }
+  // }
+
+  // predicate {:opaque} tryAdvanceLocation(cm: CM, io: IO,
+  //     cm': CM, io': IO)
+  // requires CommitterModel.Inv(cm)
+  // requires io.IOInit?
+  // requires cm.status == StatusReady
+  // requires cm.frozenLoc.Some?
+  // {
+  //   var hasFrozen := JournalistModel.hasFrozenJournal(cm.journalist);
+  //   var hasInMem := JournalistModel.hasInMemoryJournal(cm.journalist);
+  //   if cm.superblockWrite.None? then (
+  //     if hasFrozen || hasInMem then (
+  //       (cm', io') == WriteOutJournal(cm, io)
+  //     ) else if cm.outstandingJournalWrites == {} then (
+  //       writeOutSuperblockAdvanceLocation(cm, io, cm', io')
+  //     ) else (
+  //       && cm' == cm
+  //       && io' == io
+  //     )
+  //   ) else (
+  //     && cm' == cm
+  //     && io' == io
+  //   )
+  // }
+
+  // lemma tryAdvanceLocationCorrect(cm: CM, io: IO,
+  //     cm': CM, io': IO)
+  // requires CommitterModel.Inv(cm)
+  // requires io.IOInit?
+  // requires cm.status.StatusReady?
+  // requires cm.frozenLoc.Some?
+  // requires tryAdvanceLocation(cm, io, cm', io')
+  // ensures CommitterModel.WF(cm')
+  // ensures ValidDiskOp(diskOp(io'))
+  // ensures IDiskOp(diskOp(io')).bdop.NoDiskOp?
+  // ensures JC.Next(
+  //       CommitterModel.I(cm),
+  //       CommitterModel.I(cm'),
+  //       IDiskOp(diskOp(io')).jdop,
+  //       JournalInternalOp)
+  // {
+  //   reveal_tryAdvanceLocation();
+  //   var hasFrozen := JournalistModel.hasFrozenJournal(cm.journalist);
+  //   var hasInMem := JournalistModel.hasInMemoryJournal(cm.journalist);
+  //   if cm.superblockWrite.None? {
+  //     if hasFrozen || hasInMem {
+  //       WriteOutJournalCorrect(cm, io);
+  //     } else if (cm.outstandingJournalWrites == {}) {
+  //       writeOutSuperblockAdvanceLocationCorrect(cm, io, cm', io');
+  //     } else {
+  //       assert JC.NoOp( CommitterModel.I(cm), CommitterModel.I(cm'), JournalDisk.NoDiskOp, JournalInternalOp);
+  //       assert JC.NextStep( CommitterModel.I(cm), CommitterModel.I(cm'), JournalDisk.NoDiskOp, JournalInternalOp, JC.NoOpStep);
+  //     }
+  //   } else {
+  //     assert JC.NoOp( CommitterModel.I(cm), CommitterModel.I(cm'), JournalDisk.NoDiskOp, JournalInternalOp);
+  //     assert JC.NextStep( CommitterModel.I(cm), CommitterModel.I(cm'), JournalDisk.NoDiskOp, JournalInternalOp, JC.NoOpStep);
+  //   }
+  // }
+
+  // function {:opaque} writeBackSuperblockResp(
+  //     cm: CommitterModel.CM) : CommitterModel.CM
+  // requires CommitterModel.Inv(cm)
+  // {
+  //   if cm.status.StatusReady? &&
+  //       cm.commitStatus.CommitAdvanceLocation? then (
+  //     cm.(superblockWrite := None)
+  //       .(superblock := cm.newSuperblock.value)
+  //       .(newSuperblock := None)
+  //       .(whichSuperblock := if cm.whichSuperblock == 0 then 1 else 0)
+  //       .(syncReqs := SyncReqs2to1(cm.syncReqs))
+  //       .(journalist :=
+  //           JournalistModel.updateWrittenJournalLen(
+  //             cm.journalist,
+  //             JournalistModel.getWrittenJournalLen(cm.journalist)
+  //               - cm.frozenJournalPosition
+  //           )
+  //        )
+  //       .(frozenJournalPosition := 0)
+  //       .(frozenLoc := None)
+  //       .(isFrozen := false)
+  //       .(commitStatus := JC.CommitNone)
+  //   )
+  //   else if cm.status.StatusReady? &&
+  //       cm.commitStatus.CommitAdvanceLog? then (
+  //     cm.(superblockWrite := None)
+  //       .(superblock := cm.newSuperblock.value)
+  //       .(newSuperblock := None)
+  //       .(whichSuperblock := if cm.whichSuperblock == 0 then 1 else 0)
+  //       .(syncReqs := SyncReqs2to1(cm.syncReqs))
+  //       .(commitStatus := JC.CommitNone)
+  //   )
+  //   else (
+  //     cm
+  //   )
+  // }
+
+  // lemma writeBackSuperblockRespCorrect(
+  //     cm: CommitterModel.CM, io: IO)
+  // requires CommitterModel.Inv(cm)
+  // requires ValidDiskOp(diskOp(io))
+  // requires IDiskOp(diskOp(io)).jdop.RespWriteSuperblockOp?
+  // requires Some(io.id) == cm.superblockWrite
+  // ensures var cm' := writeBackSuperblockResp(cm);
+  //   && CommitterModel.WF(cm')
+  //   && JC.Next(
+  //       CommitterModel.I(cm),
+  //       CommitterModel.I(cm'),
+  //       IDiskOp(diskOp(io)).jdop,
+  //       if cm.status.StatusReady? && cm.commitStatus.CommitAdvanceLocation? then CleanUpOp else JournalInternalOp
+  //   )
+  // {
+  //   reveal_writeBackSuperblockResp();
+  //   var cm' := writeBackSuperblockResp(cm);
+  //   SyncReqs2to1Correct(cm.syncReqs);
+  //   if cm.status.StatusReady? &&
+  //       cm.commitStatus.CommitAdvanceLocation? {
+  //     assert JC.WriteBackSuperblockResp(
+  //         CommitterModel.I(cm),
+  //         CommitterModel.I(cm'),
+  //         IDiskOp(diskOp(io)).jdop,
+  //         CleanUpOp);
+  //     assert JC.NextStep(
+  //         CommitterModel.I(cm),
+  //         CommitterModel.I(cm'),
+  //         IDiskOp(diskOp(io)).jdop,
+  //         CleanUpOp,
+  //         JC.WriteBackSuperblockRespStep);
+  //   }
+  //   else if cm.status.StatusReady? &&
+  //       cm.commitStatus.CommitAdvanceLog? {
+  //     assert JC.WriteBackSuperblockResp(
+  //         CommitterModel.I(cm),
+  //         CommitterModel.I(cm'),
+  //         IDiskOp(diskOp(io)).jdop,
+  //         JournalInternalOp);
+  //     assert JC.NextStep(
+  //         CommitterModel.I(cm),
+  //         CommitterModel.I(cm'),
+  //         IDiskOp(diskOp(io)).jdop,
+  //         JournalInternalOp,
+  //         JC.WriteBackSuperblockRespStep);
+  //   }
+  //   else {
+  //     assert JC.NoOp(
+  //         CommitterModel.I(cm),
+  //         CommitterModel.I(cm'),
+  //         IDiskOp(diskOp(io)).jdop,
+  //         JournalInternalOp);
+  //     assert JC.NextStep(
+  //         CommitterModel.I(cm),
+  //         CommitterModel.I(cm'),
+  //         IDiskOp(diskOp(io)).jdop,
+  //         JournalInternalOp,
+  //         JC.NoOpStep);
+  //   }
+  // }
 }
